Runtime/Interface.lean
@@ -10,26 +10,23 @@ structure Scheme where
 attribute [reducible] Scheme.type
 attribute [instance] Scheme.varsDecidableEq
 
-abbrev Scheme.restrict (σ : Scheme) (Sub : Type) [DecidableEq Sub] [InjectiveCoe Sub σ.vars] : Scheme := {
+abbrev Scheme.restrict (σ : Scheme) (Sub : Type) [DecidableEq Sub] [InjectiveCoe Sub σ.vars] : Scheme where
   vars := Sub
-  type := fun var => σ.type var
-}
+  type var := σ.type var
 
-abbrev Scheme.union (σ₁ σ₂ : Scheme) : Scheme := {
+abbrev Scheme.union (σ₁ σ₂ : Scheme) : Scheme where
   vars := Sum σ₁.vars σ₂.vars
-  type := fun
+  type
     | .inl var => σ₁.type var 
     | .inr var => σ₂.type var
-}
 
 infix:65 " ⊎ " => Scheme.union
 
-abbrev Scheme.bUnion {Schemes : Type} [DecidableEq Schemes] (σ : Schemes → Scheme) : Scheme := {
+abbrev Scheme.bUnion {Schemes : Type} [DecidableEq Schemes] (σ : Schemes → Scheme) : Scheme where
   vars := Σ scheme : Schemes, (σ scheme).vars
   type := fun ⟨scheme, var⟩ => (σ scheme).type var
-}
 
-prefix:100 "⨄ " => Scheme.bUnion
+prefix:100 " ⨄ " => Scheme.bUnion
 
 @[reducible]
 instance {σ : Scheme} {Sub : Type} [DecidableEq Sub] [InjectiveCoe Sub σ.vars] : InjectiveCoe (σ.restrict Sub).vars σ.vars := 
@@ -43,10 +40,10 @@ abbrev _root_.Interface (σ : Interface.Scheme) := (var : σ.vars) → Option (�
 def empty : Interface σ := fun _ => none
 
 def isPresent (i : Interface σ) (var : σ.vars) : Bool :=
-  (i var).isSome
+  i var |>.isSome
 
 -- Merge i₂ into i₁.
 def merge (i₁ i₂ : Interface σ) : Interface σ :=
-  fun var => (i₂ var).orElse (fun _ => i₁ var)
+  fun var => i₂ var |>.orElse fun _ => i₁ var
 
 end Interface
