Runtime/Utilities.lean
@@ -1,3 +1,2 @@
 import Runtime.Utilities.Extensions
 import Runtime.Utilities.SortedArray
-import Runtime.Utilities.Tree
